Examples/SignedDH/Instance.lean
@@ -1,0 +1,312 @@
+module
+
+public import Examples.SignedDH.Specification
+public import Examples.SignedDH.Proof
+
+namespace DY.Example.SignedDH
+
+public section
+
+abbrev SubF.internal: (id: Fin 6) → (Type → Type)
+  | 0 => Literal.SubF
+  | 1 => Concat.SubF
+  | 2 => Hash.SubF
+  | 3 => Signature.SubF
+  | 4 => DiffieHellman.SubF
+  | 5 => Random.SubF
+
+abbrev SubF := BytesFunctor.combine SubF.internal
+
+instance: ∀ id, SubBytesFunctor (SubF.internal id)
+  | 0 | 1 | 2 | 3 | 4 | 5 => inferInstance
+
+instance: BytesFunctor.HasStep Literal.SubF SubF := inferInstanceAs (BytesFunctor.HasStep (SubF.internal 0) SubF)
+instance: BytesFunctor.HasStep Concat.SubF SubF := inferInstanceAs (BytesFunctor.HasStep (SubF.internal 1) SubF)
+instance: BytesFunctor.HasStep Hash.SubF SubF := inferInstanceAs (BytesFunctor.HasStep (SubF.internal 2) SubF)
+instance: BytesFunctor.HasStep Signature.SubF SubF := inferInstanceAs (BytesFunctor.HasStep (SubF.internal 3) SubF)
+instance: BytesFunctor.HasStep DiffieHellman.SubF SubF := inferInstanceAs (BytesFunctor.HasStep (SubF.internal 4) SubF)
+instance: BytesFunctor.HasStep Random.SubF SubF := inferInstanceAs (BytesFunctor.HasStep (SubF.internal 5) SubF)
+
+instance: BytesFunctor where
+  BytesF := SubF
+
+instance: BytesFunctor.Has SubF := inferInstanceAs (BytesFunctor.Has BytesF)
+
+example: BytesFunctor.Has Hash.SubF := inferInstance
+example: BytesFunctor.Has Signature.SubF := inferInstance
+example: BytesFunctor.Has DiffieHellman.SubF := inferInstance
+example: BytesFunctor.Has Random.SubF := inferInstance
+
+def SubF.length.internal [BytesFunctor]: ∀ id, Bytes.PartialLength (SubF.internal id)
+  | 0 => Literal.SubF.length
+  | 1 => Concat.SubF.length
+  | 2 => Hash.SubF.length
+  | 3 => Signature.SubF.length
+  | 4 => DiffieHellman.SubF.length
+  | 5 => Random.SubF.length
+
+abbrev SubF.length [BytesFunctor]: Bytes.PartialLength SubF :=
+  Bytes.PartialLength.combine SubF.length.internal
+
+instance: BytesLength where
+  funs := SubF.length
+
+instance: BytesLength.HasStep Literal.SubF.length SubF.length := inferInstanceAs (BytesLength.HasStep (SubF.length.internal 0) SubF.length)
+instance: BytesLength.HasStep Concat.SubF.length SubF.length := inferInstanceAs (BytesLength.HasStep (SubF.length.internal 1) SubF.length)
+instance: BytesLength.HasStep Hash.SubF.length SubF.length := inferInstanceAs (BytesLength.HasStep (SubF.length.internal 2) SubF.length)
+instance: BytesLength.HasStep Signature.SubF.length SubF.length := inferInstanceAs (BytesLength.HasStep (SubF.length.internal 3) SubF.length)
+instance: BytesLength.HasStep DiffieHellman.SubF.length SubF.length := inferInstanceAs (BytesLength.HasStep (SubF.length.internal 4) SubF.length)
+instance: BytesLength.HasStep Random.SubF.length SubF.length := inferInstanceAs (BytesLength.HasStep (SubF.length.internal 5) SubF.length)
+
+instance: BytesLength.Has SubF.length := inferInstanceAs (BytesLength.Has SubF.length)
+
+example: BytesLength.Has Literal.SubF.length := inferInstance
+example: BytesLength.Has Concat.SubF.length := inferInstance
+example: BytesLength.Has Hash.SubF.length := inferInstance
+example: BytesLength.Has Signature.SubF.length := inferInstance
+example: BytesLength.Has DiffieHellman.SubF.length := inferInstance
+example: BytesLength.Has Random.SubF.length := inferInstance
+
+def attackerKnowledge.internal (id: Fin 6): SubAttackerKnowledge (SubF.internal id) :=
+  match id with
+  | 0 => Literal.attackerKnowledge
+  | 1 => Concat.attackerKnowledge
+  | 2 => Hash.attackerKnowledge
+  | 3 => Signature.attackerKnowledge
+  | 4 => DiffieHellman.attackerKnowledge
+  | 5 => Random.attackerKnowledge
+
+def attackerKnowledge: SubAttackerKnowledge SubF :=
+  SubAttackerKnowledge.combine attackerKnowledge.internal
+
+instance: AttackerKnowledge.HasStep Literal.attackerKnowledge attackerKnowledge := inferInstanceAs (AttackerKnowledge.HasStep (attackerKnowledge.internal 0) (SubAttackerKnowledge.combine attackerKnowledge.internal))
+instance: AttackerKnowledge.HasStep Concat.attackerKnowledge attackerKnowledge := inferInstanceAs (AttackerKnowledge.HasStep (attackerKnowledge.internal 1) (SubAttackerKnowledge.combine attackerKnowledge.internal))
+instance: AttackerKnowledge.HasStep Hash.attackerKnowledge attackerKnowledge := inferInstanceAs (AttackerKnowledge.HasStep (attackerKnowledge.internal 2) (SubAttackerKnowledge.combine attackerKnowledge.internal))
+instance: AttackerKnowledge.HasStep Signature.attackerKnowledge attackerKnowledge := inferInstanceAs (AttackerKnowledge.HasStep (attackerKnowledge.internal 3) (SubAttackerKnowledge.combine attackerKnowledge.internal))
+instance: AttackerKnowledge.HasStep DiffieHellman.attackerKnowledge attackerKnowledge := inferInstanceAs (AttackerKnowledge.HasStep (attackerKnowledge.internal 4) (SubAttackerKnowledge.combine attackerKnowledge.internal))
+instance: AttackerKnowledge.HasStep Random.attackerKnowledge attackerKnowledge := inferInstanceAs (AttackerKnowledge.HasStep (attackerKnowledge.internal 5) (SubAttackerKnowledge.combine attackerKnowledge.internal))
+
+instance: AttackerKnowledge where
+  attackerKnowledge
+
+instance: AttackerKnowledge.Has attackerKnowledge := inferInstanceAs (AttackerKnowledge.Has AttackerKnowledge.attackerKnowledge)
+
+example: AttackerKnowledge.Has Hash.attackerKnowledge := inferInstance
+example: AttackerKnowledge.Has Signature.attackerKnowledge := inferInstance
+example: AttackerKnowledge.Has DiffieHellman.attackerKnowledge := inferInstance
+example: AttackerKnowledge.Has Random.attackerKnowledge := inferInstance
+
+instance: HasExecBytes where
+
+public
+abbrev ExecEntryT.internal: Fin 7 → Type
+  | 0 => Network.ExecEntryT
+  | 1 => Random.ExecEntryT
+  | 2 => ProtocolEvent.ExecEntryT SignedDH.SignedDHEvent
+  | 3 => PersistentLocalState.CompromisableState.ExecEntryT SignedDH.ClientInitiateState
+  | 4 => PersistentLocalState.CompromisableState.ExecEntryT SignedDH.ClientFinishState
+  | 5 => PersistentLocalState.CompromisableState.ExecEntryT SignedDH.ServerFinishState
+  | 6 => LongTermKeys.ExecEntryT "SignedDH"
+
+public
+abbrev ExecEntryT: Type :=
+  ExecTraceTypes.combine ExecEntryT.internal
+
+instance: ExecTraceTypes.HasStep Network.ExecEntryT ExecEntryT := inferInstanceAs (ExecTraceTypes.HasStep (ExecEntryT.internal 0) (ExecTraceTypes.combine ExecEntryT.internal))
+instance: ExecTraceTypes.HasStep Random.ExecEntryT ExecEntryT := inferInstanceAs (ExecTraceTypes.HasStep (ExecEntryT.internal 1) (ExecTraceTypes.combine ExecEntryT.internal))
+instance: ExecTraceTypes.HasStep (ProtocolEvent.ExecEntryT SignedDH.SignedDHEvent) ExecEntryT := inferInstanceAs (ExecTraceTypes.HasStep (ExecEntryT.internal 2) (ExecTraceTypes.combine ExecEntryT.internal))
+instance: ExecTraceTypes.HasStep (PersistentLocalState.CompromisableState.ExecEntryT SignedDH.ClientInitiateState) ExecEntryT := inferInstanceAs (ExecTraceTypes.HasStep (ExecEntryT.internal 3) (ExecTraceTypes.combine ExecEntryT.internal))
+instance: ExecTraceTypes.HasStep (PersistentLocalState.CompromisableState.ExecEntryT SignedDH.ClientFinishState) ExecEntryT := inferInstanceAs (ExecTraceTypes.HasStep (ExecEntryT.internal 4) (ExecTraceTypes.combine ExecEntryT.internal))
+instance: ExecTraceTypes.HasStep (PersistentLocalState.CompromisableState.ExecEntryT SignedDH.ServerFinishState) ExecEntryT := inferInstanceAs (ExecTraceTypes.HasStep (ExecEntryT.internal 5) (ExecTraceTypes.combine ExecEntryT.internal))
+instance: ExecTraceTypes.HasStep (LongTermKeys.ExecEntryT "SignedDH") ExecEntryT := inferInstanceAs (ExecTraceTypes.HasStep (ExecEntryT.internal 6) (ExecTraceTypes.combine ExecEntryT.internal))
+
+instance: ExecTraceTypes where
+  ExecT := ExecEntryT
+
+instance: ExecTraceTypes.Has ExecEntryT := inferInstanceAs (ExecTraceTypes.Has ExecTrace.Entry)
+
+example: ExecTraceTypes.Has Network.ExecEntryT := inferInstance
+example: ExecTraceTypes.Has Random.ExecEntryT := inferInstance
+example: ExecTraceTypes.Has (ProtocolEvent.ExecEntryT SignedDH.SignedDHEvent) := inferInstance
+example: ExecTraceTypes.Has (PersistentLocalState.CompromisableState.ExecEntryT SignedDH.ClientInitiateState) := inferInstance
+example: ExecTraceTypes.Has (PersistentLocalState.CompromisableState.ExecEntryT SignedDH.ClientFinishState) := inferInstance
+example: ExecTraceTypes.Has (PersistentLocalState.CompromisableState.ExecEntryT SignedDH.ServerFinishState) := inferInstance
+example: ExecTraceTypes.Has (LongTermKeys.ExecEntryT "SignedDH") := inferInstance
+
+public
+def baseAttackerKnowledge.internal: (id: Fin 7) → SubBaseAttackerKnowledge (ExecEntryT.internal id)
+  | 0 => Network.baseAttackerKnowledge
+  | 1 => Random.baseAttackerKnowledge
+  | 2 => ProtocolEvent.baseAttackerKnowledge SignedDH.SignedDHEvent
+  | 3 => PersistentLocalState.CompromisableState.baseAttackerKnowledge SignedDH.ClientInitiateState
+  | 4 => PersistentLocalState.CompromisableState.baseAttackerKnowledge SignedDH.ClientFinishState
+  | 5 => PersistentLocalState.CompromisableState.baseAttackerKnowledge SignedDH.ServerFinishState
+  | 6 => LongTermKeys.baseAttackerKnowledge "SignedDH"
+
+public
+def baseAttackerKnowledge: SubBaseAttackerKnowledge ExecEntryT :=
+  SubBaseAttackerKnowledge.combine baseAttackerKnowledge.internal
+
+instance: BaseAttackerKnowledge where
+  attackerKnows := baseAttackerKnowledge
+
+instance: HasExecTrace where
+
+@[expose]
+public
+def ProofEntryT.internal: Fin 7 → Type
+  | 0 => Network.ProofEntryT
+  | 1 => Random.ProofEntryT
+  | 2 => ProtocolEvent.ProofEntryT SignedDH.SignedDHEvent
+  | 3 => PersistentLocalState.CompromisableState.ProofEntryT SignedDH.ClientInitiateState
+  | 4 => PersistentLocalState.CompromisableState.ProofEntryT SignedDH.ClientFinishState
+  | 5 => PersistentLocalState.CompromisableState.ProofEntryT SignedDH.ServerFinishState
+  | 6 => LongTermKeys.ProofEntryT "SignedDH"
+
+public
+abbrev ProofEntryT: Type :=
+  ProofTraceTypes.combine ProofEntryT.internal
+
+public
+instance: ∀ id, ErasableProofEntry (ExecEntryT.internal id) (ProofEntryT.internal id)
+  | 0 | 1 | 2 | 3 | 4 | 5 | 6 => by dsimp only [ExecEntryT.internal, ProofEntryT.internal]; infer_instance
+
+public
+instance: ErasableProofEntry ExecEntryT ProofEntryT :=
+  (inferInstance: ErasableProofEntry (ExecTraceTypes.combine ExecEntryT.internal) (ProofTraceTypes.combine ProofEntryT.internal))
+
+instance: ProofTraceTypes.HasStep Network.ProofEntryT ProofEntryT := inferInstanceAs (ProofTraceTypes.HasStep (ProofEntryT.internal 0) (ProofTraceTypes.combine ProofEntryT.internal))
+instance: ProofTraceTypes.HasStep Random.ProofEntryT ProofEntryT := inferInstanceAs (ProofTraceTypes.HasStep (ProofEntryT.internal 1) (ProofTraceTypes.combine ProofEntryT.internal))
+instance: ProofTraceTypes.HasStep (ProtocolEvent.ProofEntryT SignedDH.SignedDHEvent) ProofEntryT := inferInstanceAs (ProofTraceTypes.HasStep (ProofEntryT.internal 2) (ProofTraceTypes.combine ProofEntryT.internal))
+instance: ProofTraceTypes.HasStep (PersistentLocalState.CompromisableState.ProofEntryT SignedDH.ClientInitiateState) ProofEntryT := inferInstanceAs (ProofTraceTypes.HasStep (ProofEntryT.internal 3) (ProofTraceTypes.combine ProofEntryT.internal))
+instance: ProofTraceTypes.HasStep (PersistentLocalState.CompromisableState.ProofEntryT SignedDH.ClientFinishState) ProofEntryT := inferInstanceAs (ProofTraceTypes.HasStep (ProofEntryT.internal 4) (ProofTraceTypes.combine ProofEntryT.internal))
+instance: ProofTraceTypes.HasStep (PersistentLocalState.CompromisableState.ProofEntryT SignedDH.ServerFinishState) ProofEntryT := inferInstanceAs (ProofTraceTypes.HasStep (ProofEntryT.internal 5) (ProofTraceTypes.combine ProofEntryT.internal))
+instance: ProofTraceTypes.HasStep (LongTermKeys.ProofEntryT "SignedDH") ProofEntryT := inferInstanceAs (ProofTraceTypes.HasStep (ProofEntryT.internal 6) (ProofTraceTypes.combine ProofEntryT.internal))
+
+instance: ProofTraceTypes where
+  ProofT := ProofEntryT
+  tc := inferInstance
+
+instance: ProofTraceTypes.Has ProofEntryT := inferInstanceAs (ProofTraceTypes.Has ProofTrace.Entry)
+
+example: ProofTraceTypes.Has Network.ProofEntryT := inferInstance
+example: ProofTraceTypes.Has Random.ProofEntryT := inferInstance
+example: ProofTraceTypes.Has (ProtocolEvent.ProofEntryT SignedDH.SignedDHEvent) := inferInstance
+example: ProofTraceTypes.Has (PersistentLocalState.CompromisableState.ProofEntryT SignedDH.ClientInitiateState) := inferInstance
+example: ProofTraceTypes.Has (PersistentLocalState.CompromisableState.ProofEntryT SignedDH.ClientFinishState) := inferInstance
+example: ProofTraceTypes.Has (PersistentLocalState.CompromisableState.ProofEntryT SignedDH.ServerFinishState) := inferInstance
+example: ProofTraceTypes.Has (LongTermKeys.ProofEntryT "SignedDH") := inferInstance
+
+instance: HasProofTrace where
+
+def invariants.internal: (id: Fin 6) → Bytes.PartialInvariants (SubF.internal id)
+  | 0 => Literal.invariants
+  | 1 => Concat.invariants
+  | 2 => Hash.invariants
+  | 3 => Signature.invariants
+  | 4 => DiffieHellman.invariants
+  | 5 => Random.invariants
+
+abbrev invariants: Bytes.PartialInvariants SubF :=
+  Bytes.PartialInvariants.combine invariants.internal
+
+instance [BytesInvariants]: BytesInvariants.HasStep Literal.invariants invariants := inferInstanceAs (BytesInvariants.HasStep (invariants.internal 0) invariants)
+instance [BytesInvariants]: BytesInvariants.HasStep Concat.invariants invariants := inferInstanceAs (BytesInvariants.HasStep (invariants.internal 1) invariants)
+instance [BytesInvariants]: BytesInvariants.HasStep Hash.invariants invariants := inferInstanceAs (BytesInvariants.HasStep (invariants.internal 2) invariants)
+instance [BytesInvariants]: BytesInvariants.HasStep Signature.invariants invariants := inferInstanceAs (BytesInvariants.HasStep (invariants.internal 3) invariants)
+instance [BytesInvariants]: BytesInvariants.HasStep DiffieHellman.invariants invariants := inferInstanceAs (BytesInvariants.HasStep (invariants.internal 4) invariants)
+instance [BytesInvariants]: BytesInvariants.HasStep Random.invariants invariants := inferInstanceAs (BytesInvariants.HasStep (invariants.internal 5) invariants)
+
+instance: BytesInvariants where
+  invs := invariants
+
+instance: BytesInvariants.Has invariants := inferInstance
+
+example: BytesInvariants.Has Hash.invariants := inferInstance
+example: BytesInvariants.Has Signature.invariants := inferInstance
+example: BytesInvariants.Has DiffieHellman.invariants := inferInstance
+example: BytesInvariants.Has Random.invariants := inferInstance
+
+def invariantsProofs.internal: (id: Fin 6) → Bytes.PartialInvariantsProofs (invariants.internal id)
+  | 0 => Literal.invariantsProofs
+  | 1 => Concat.invariantsProofs
+  | 2 => Hash.invariantsProofs
+  | 3 => Signature.invariantsProofs
+  | 4 => DiffieHellman.invariantsProofs
+  | 5 => Random.invariantsProofs
+
+abbrev invariantsProofs: Bytes.PartialInvariantsProofs invariants :=
+  Bytes.PartialInvariantsProofs.combine invariantsProofs.internal
+
+instance: BytesInvariantsProofs where
+  pfs := invariantsProofs
+
+instance: HasBytesInvariants where
+
+public
+instance: ∀ id, SubTraceInvariant (ProofEntryT.internal id)
+  | 0 | 1 | 2 | 3 | 4 | 5 | 6 => by dsimp only [ProofEntryT.internal]; infer_instance
+
+public
+instance: SubTraceInvariant ProofEntryT :=
+  (inferInstance: SubTraceInvariant (ProofTraceTypes.combine ProofEntryT.internal))
+
+instance : TraceInvariant where
+  tc_inv := by dsimp only [ProofTrace.Entry, ProofTraceTypes.ProofT]; infer_instance
+
+instance: TraceInvariant.Has ProofEntryT := inferInstanceAs (TraceInvariant.Has ProofTrace.Entry)
+
+instance: TraceInvariant.HasStep Network.ProofEntryT ProofEntryT := inferInstanceAs (TraceInvariant.HasStep (ProofEntryT.internal 0) (ProofTraceTypes.combine ProofEntryT.internal))
+instance: TraceInvariant.HasStep Random.ProofEntryT ProofEntryT := inferInstanceAs (TraceInvariant.HasStep (ProofEntryT.internal 1) (ProofTraceTypes.combine ProofEntryT.internal))
+instance: TraceInvariant.HasStep (ProtocolEvent.ProofEntryT SignedDH.SignedDHEvent) ProofEntryT := inferInstanceAs (TraceInvariant.HasStep (ProofEntryT.internal 2) (ProofTraceTypes.combine ProofEntryT.internal))
+instance: TraceInvariant.HasStep (PersistentLocalState.CompromisableState.ProofEntryT SignedDH.ClientInitiateState) ProofEntryT := inferInstanceAs (TraceInvariant.HasStep (ProofEntryT.internal 3) (ProofTraceTypes.combine ProofEntryT.internal))
+instance: TraceInvariant.HasStep (PersistentLocalState.CompromisableState.ProofEntryT SignedDH.ClientFinishState) ProofEntryT := inferInstanceAs (TraceInvariant.HasStep (ProofEntryT.internal 4) (ProofTraceTypes.combine ProofEntryT.internal))
+instance: TraceInvariant.HasStep (PersistentLocalState.CompromisableState.ProofEntryT SignedDH.ServerFinishState) ProofEntryT := inferInstanceAs (TraceInvariant.HasStep (ProofEntryT.internal 5) (ProofTraceTypes.combine ProofEntryT.internal))
+instance: TraceInvariant.HasStep (LongTermKeys.ProofEntryT "SignedDH") ProofEntryT := inferInstanceAs (TraceInvariant.HasStep (ProofEntryT.internal 6) (ProofTraceTypes.combine ProofEntryT.internal))
+
+example: TraceInvariant.Has Network.ProofEntryT := inferInstance
+example: TraceInvariant.Has Random.ProofEntryT := inferInstance
+example: TraceInvariant.Has (ProtocolEvent.ProofEntryT SignedDH.SignedDHEvent) := inferInstance
+example: TraceInvariant.Has (PersistentLocalState.CompromisableState.ProofEntryT SignedDH.ClientInitiateState) := inferInstance
+example: TraceInvariant.Has (PersistentLocalState.CompromisableState.ProofEntryT SignedDH.ClientFinishState) := inferInstance
+example: TraceInvariant.Has (PersistentLocalState.CompromisableState.ProofEntryT SignedDH.ServerFinishState) := inferInstance
+example: TraceInvariant.Has (LongTermKeys.ProofEntryT "SignedDH") := inferInstance
+
+instance : ∀ id, SubBaseAttackerKnowledgeTheorem (ProofEntryT.internal id) (baseAttackerKnowledge.internal id)
+  -- TODO: investigate why infer_instance doesn't work
+  | 0 => by dsimp only [ProofEntryT.internal, baseAttackerKnowledge.internal]; apply Network.baseAttackerKnowledgeTheorem
+  | 1 => by dsimp only [ProofEntryT.internal, baseAttackerKnowledge.internal]; apply Random.baseAttackerKnowledgeTheorem
+  | 2 => by dsimp only [ProofEntryT.internal, baseAttackerKnowledge.internal]; apply ProtocolEvent.baseAttackerKnowledgeTheorem
+  | 3 => by dsimp only [ProofEntryT.internal, baseAttackerKnowledge.internal]; apply PersistentLocalState.CompromisableState.baseAttackerKnowledgeTheorem
+  | 4 => by dsimp only [ProofEntryT.internal, baseAttackerKnowledge.internal]; apply PersistentLocalState.CompromisableState.baseAttackerKnowledgeTheorem
+  | 5 => by dsimp only [ProofEntryT.internal, baseAttackerKnowledge.internal]; apply PersistentLocalState.CompromisableState.baseAttackerKnowledgeTheorem
+  | 6 => by dsimp only [ProofEntryT.internal, baseAttackerKnowledge.internal]; apply LongTermKeys.baseAttackerKnowledgeTheorem "SignedDH"
+
+instance: SubBaseAttackerKnowledgeTheorem (ProofEntryT) (baseAttackerKnowledge) := by
+  dsimp only [ProofEntryT, baseAttackerKnowledge]
+  infer_instance
+
+instance: BaseAttackerKnowledgeTheorem where
+  pf := by
+    dsimp only [ProofTrace.Entry, ProofTraceTypes.ProofT, BaseAttackerKnowledge.attackerKnows]
+    -- TODO infer_instance
+    exact instSubBaseAttackerKnowledgeTheoremExecEntryTProofEntryTBaseAttackerKnowledge
+
+instance: (id: Fin 6) → SubAttackerKnowledgeTheorem (attackerKnowledge.internal id)
+  | 0 => inferInstanceAs (SubAttackerKnowledgeTheorem Literal.attackerKnowledge)
+  | 1 => inferInstanceAs (SubAttackerKnowledgeTheorem Concat.attackerKnowledge)
+  | 2 => inferInstanceAs (SubAttackerKnowledgeTheorem Hash.attackerKnowledge)
+  | 3 => inferInstanceAs (SubAttackerKnowledgeTheorem Signature.attackerKnowledge)
+  | 4 => inferInstanceAs (SubAttackerKnowledgeTheorem DiffieHellman.attackerKnowledge)
+  | 5 => inferInstanceAs (SubAttackerKnowledgeTheorem Random.attackerKnowledge)
+
+instance: SubAttackerKnowledgeTheorem attackerKnowledge := inferInstanceAs (SubAttackerKnowledgeTheorem (SubAttackerKnowledge.combine attackerKnowledge.internal))
+
+instance: AttackerKnowledgeTheorem where
+  inst := inferInstanceAs (SubAttackerKnowledgeTheorem attackerKnowledge)
+
+instance: HasTraceInvariant where
+
+end
+
+end DY.Example.SignedDH
